thy/Iptables_Semantics/Common/RepeatStabilize.thy
@@ -19,5 +19,10 @@ lemma repeat_stabilize_funpow: "repeat_stabilize n f v = (f^^n) v"
   qed(simp)
 
 
+lemma repeat_stabilize_induct: "(P m) \<Longrightarrow> (\<And>m. P m \<Longrightarrow> P (f m)) \<Longrightarrow> P (repeat_stabilize n f m)"
+  apply(simp add: repeat_stabilize_funpow)
+  apply(induction n)
+   by(simp)+  
+
 
 end
